\uuid{2957}
\titre{$\sum 2^{-k}/\cos\theta\dots\cos(2^k\theta)$}
\theme{}
\auteur{quercia}
\date{2010/03/08}
\organisation{exo7}
\contenu{
  \texte{}
  \question{Simplifier $$\sum_{k=1}^n\, \frac 1
{2^k \cos\theta \cos2\theta \cos4\theta \dots \cos2^{k-1}\theta}.$$}
  \reponse{$S = \frac {u-u^{-1}}{u^2-u^{-2}} +
     \frac {u-u^{-1}}{u^4-u^{-4}} + \dots +
     \frac {u-u^{-1}}{u^{2^n}-u^{-2^n}}$.
\par
$\frac {u-u^{-1}}{u^2-u^{-2}} +
 \frac {u-u^{-1}}{u^4-u^{-4}} =
 \frac {u^3-u^{-3}}{u^4-u^{-4}}$.
\par
$\frac {u^3-u^{-3}}{u^4-u^{-4}} +
 \frac {u-u^{-1}}{u^8-u^{-8}} =
 \frac {u^7-u^{-7}}{u^8-u^{-8}}$
$\ldots$
\par
$ \Rightarrow  S = \frac {u^{2^n-1}-u^{-2^n+1}}{u^{2^n}-u^{-2^n}}
       = \frac {\sin\bigl((2^n-1)\theta\bigr)}{\sin(2^n\theta)}$.}
}