\uuid{3968}
\titre{Dérivée $n$-ème de $x^n(1-x)^n$}
\theme{}
\auteur{quercia}
\date{2010/03/11}
\organisation{exo7}
\contenu{
  \texte{}
  \question{Calculer la dérivée $n^{\text{ème}}$ de $x \mapsto x^n(1-x)^n$.
En déduire la valeur de $\sum_{k=0}^n \bigl(C_n^k\bigr)^2$.}
  \reponse{$\frac{d^n}{d x^n}\bigl(x^n(1-x)^n\bigr) =
         \sum_{k=0}^n n!\,\bigl(C_n^k\bigr)^2 (-1)^{n-k} x^{n-k}(1-x)^k$.
         \par
         coefficient de $x^n = (-1)^n n!\, \sum_{k=0}^n \bigl(C_n^k\bigr)^2
                             = (-1)^n A_{2n}^n$.}
}